HW6 completed

hw6/Homework6.dfy
@@ -2,28 +2,78 @@ datatype Tree<T> = Leaf | Node(Tree<T>, Tree<T>, T)
 datatype List<T> = Nil | Cons(T, List<T>)
 
 function flatten<T>(tree:Tree<T>):List<T>
+decreases tree
+ensures tree==Leaf ==> flatten(tree)==Nil
 {
-	
+  match tree
+  case Leaf                  => Nil
+  case Node (left, right, m) => append(Cons(m, flatten(left)), flatten(right)) 
 }
 
 function append<T>(xs:List<T>, ys:List<T>):List<T>
+decreases xs, ys
+ensures xs==Nil ==> append(xs, ys)==ys
+ensures ys == Nil ==> append(xs, ys)==xs
 {
-	
+  match xs
+  case  Nil => ys
+  case Cons(x, xs') => Cons(x, append(xs', ys))
 }
 
 function treeContains<T>(tree:Tree<T>, element:T):bool
+decreases tree
 {
-	
+  match tree
+  case  Leaf => false
+  case  Node (left, right, m) => m==element || treeContains(left, element) || treeContains(right, element)
 }
 
 function listContains<T>(xs:List<T>, element:T):bool
+decreases xs
 {
-	
+  match xs
+  case  Nil => false
+  case  Cons(x, xs') => x == element || listContains(xs', element)
 }
 
+lemma {:induction xs, ys} memberOfAppendOnList<T>(xs:List<T>, ys:List<T>, element:T)
+decreases xs, ys
+ensures listContains(xs, element) || listContains(ys, element) <==> listContains(append(xs, ys), element)
+{
+  match (xs) {
+    case Nil => {}
+    case Cons(x, xs') => {
+      memberOfAppendOnList(xs', ys, element);
+      assert listContains(append(xs, ys), element)
+          == listContains(append(Cons(x, xs'), ys), element)
+          == listContains(Cons(x, append(xs', ys)), element)
+          == (x == element || listContains(append(xs', ys), element))
+          == (x == element || listContains(xs', element) || listContains(ys, element))
+          == listContains(xs, element) || listContains(ys, element);
+    }
+  }
+}
 
-lemma sameElements<T>(tree:Tree<T>, element:T)
+lemma {:induction tree} sameElements<T>(tree:Tree<T>, element:T)
+decreases tree
 ensures treeContains(tree, element) <==> listContains(flatten(tree), element)
 {
-	
+  match (tree) {
+    case Leaf => {}
+    case Node(left, right, m) => {
+      sameElements(left, element);
+      sameElements(right, element);
+      assert treeContains(tree, element)
+          == treeContains(Node(left, right, m), element)
+          == (m == element || treeContains(left, element) || treeContains(right, element))
+          == (m == element || listContains(flatten(left), element) || listContains(flatten(right), element))
+          == (listContains(Cons(m, flatten(left)), element) || listContains(flatten(right), element));
+
+          memberOfAppendOnList(Cons(m, flatten(left)), flatten(right), element);
+
+      assert (listContains(Cons(m, flatten(left)), element) || listContains(flatten(right), element))
+          == listContains(append(Cons(m, flatten(left)), flatten(right)), element)
+          == listContains(flatten(tree), element);
+    }
+  }
 }
